ApplyIsAssociative and int Messages

disk-betree/Message.dfy
@@ -24,6 +24,54 @@ abstract module Message {
 	lemma DeltaIsAssociative(a: Delta, b: Delta, c: Delta)
 		ensures CombineDeltas(CombineDeltas(a, b), c) == CombineDeltas(a, CombineDeltas(b, c))
 
+	lemma ApplyIsAssociative(a: Delta, b: Delta, value: Value)
+		ensures ApplyDelta(CombineDeltas(a, b), value) == ApplyDelta(a, ApplyDelta(b, value))
+
 	lemma MergeIsAssociative(a: Message, b: Message, c: Message)
 		ensures Merge(Merge(a, b), c) == Merge(a, Merge(b, c))
+		{
+			match (a, b, c) {
+				case (Define(a), _, _) => { }
+				case (Update(a), Define(b), _) => { }
+				case (Update(a), Update(b), Define(c)) => {
+					ApplyIsAssociative(a, b, c);
+				}
+				case (Update(a), Update(b), Update(c)) => {
+					DeltaIsAssociative(a, b, c);
+				}
+			}
+		}
 }
+
+module IntMessage refines Message {
+	type Value = int
+	type Delta = int	
+
+	function NopDelta() : Delta {
+		0
+	}
+
+	function DefaultValue() : Value {
+		0
+	}
+
+	function CombineDeltas(newdelta: Delta, olddelta: Delta) : Delta {
+		newdelta + olddelta
+	}
+
+	function ApplyDelta(delta: Delta, value: Value) : Value {
+		value + delta
+	}
+
+	lemma DeltaIsAssociative(a: Delta, b: Delta, c: Delta)
+		ensures CombineDeltas(CombineDeltas(a, b), c) == CombineDeltas(a, CombineDeltas(b, c))
+		{ }
+
+	lemma ApplyIsAssociative(a: Delta, b: Delta, value: Value)
+		ensures ApplyDelta(CombineDeltas(a, b), value) == ApplyDelta(a, ApplyDelta(b, value))
+		{ }
+}
+
+
+
+
